coq/seq_ext.v
@@ -1,6 +1,6 @@
 Require Import
   Ssreflect.ssreflect Ssreflect.ssrfun Ssreflect.ssrbool
-  Ssreflect.ssrnat Ssreflect.seq.
+  Ssreflect.ssrnat Ssreflect.seq LCAC.ssrnat_ext.
 
 Set Implicit Arguments.
 
@@ -9,19 +9,14 @@ Fixpoint Forall A (P : A -> Prop) xs :=
 
 Section Seq.
 
-Variable (A : Type).
-
-Fixpoint nthopt (xs : seq A) n :=
-  if xs is x :: xs
-    then (if n is n.+1 then nthopt xs n else Some x)
-    else None.
+Variable (A B : Type).
 
 (* drop and take *)
 
 Theorem drop_addn :
   forall n m (xs : seq A), drop n (drop m xs) = drop (n + m) xs.
 Proof.
-  move => n; elim => [| m IH]; case => // x xs.
+  move => n; elim => [| m IH] [] // x xs.
   - by rewrite addn0.
   - by rewrite addnS /= IH.
 Qed.
@@ -29,26 +24,134 @@ Qed.
 Theorem take_minn :
   forall n m (xs : seq A), take n (take m xs) = take (minn n m) xs.
 Proof.
-  elim => [| n IH]; case => [| m]; case => [| x xs] => //.
-  by rewrite minnSS /=; f_equal.
+  by elim => [| n IH] [| m] [] // x xs; rewrite minnSS /= IH.
 Qed.
 
 Theorem drop_take_distr :
   forall n m (xs : seq A), drop n (take m xs) = take (m - n) (drop n xs).
 Proof.
-  elim => [| n IH]; case => [| m]; case => [| x xs] => //=.
-  - by rewrite sub0n take0.
-  - by rewrite subSS.
+  elim.
+  - by move => m xs; rewrite !drop0 subn0.
+  - move => n IH [].
+    - by move => xs; rewrite sub0n !take0.
+    - by move => m [] //= _ xs; rewrite subSS IH.
+Qed.
+
+Theorem take_drop_distr :
+  forall n m (xs : seq A), take n (drop m xs) = drop m (take (n + m) xs).
+Proof.
+  by move => n m xs; rewrite drop_take_distr addnK.
 Qed.
 
 Theorem drop_take_nil : forall n (xs : seq A), drop n (take n xs) = [::].
 Proof.
-  by move => n xs; rewrite drop_take_distr -(addn0 n) subnDl take0.
+  by move => n xs; rewrite drop_take_distr subnn take0.
 Qed.
 
 Theorem size_take : forall n (xs : seq A), size (take n xs) = minn n (size xs).
 Proof.
-  by elim => [| n IH]; case => //= x xs; rewrite IH minnSS.
+  elim.
+  - by move => xs; rewrite take0 min0n.
+  - by move => n IH [] //= _ xs; rewrite IH minnSS.
+Qed.
+
+(* nth *)
+
+Theorem nth_map' :
+  forall (f : A -> B) x xs n, f (nth x xs n) = nth (f x) (map f xs) n.
+Proof.
+  move => f x; elim => /=.
+  - by move => n; rewrite !nth_nil.
+  - by move => x' xs IH [].
+Qed.
+
+Theorem nth_equal :
+  forall (a b : A) xs n, (size xs <= n -> a = b) -> nth a xs n = nth b xs n.
+Proof.
+  move => a b; elim.
+  by move => n /= ->.
+  by move => x xs IH [].
+Qed.
+
+(* context *)
+
+Definition context := (seq (option A)).
+
+Notation ctxindex xs n x := (Some x = nth None xs n).
+Notation ctxleq xs ys := (forall n a, ctxindex xs n a -> ctxindex ys n a).
+
+Fixpoint ctxinsert xs ys n : context :=
+  if n is n.+1
+    then head None ys :: ctxinsert xs (behead ys) n
+    else xs ++ ys.
+
+Theorem size_ctxinsert :
+  forall xs ys n, size (ctxinsert xs ys n) = size xs + maxn n (size ys).
+Proof.
+  move => xs; elim => [| y ys IH].
+  - move => n.
+    rewrite /= maxn0.
+    elim: n xs => /=.
+    - by move => xs; rewrite cats0 addn0.
+    - by move => n IH xs; rewrite IH addnS.
+  - case.
+    - by rewrite /= size_cat max0n.
+    - by move => n; rewrite /= maxnSS addnS IH.
+Qed.
+
+Theorem ctxnth_ctxinsert :
+  forall xs ys n m,
+  nth None (ctxinsert xs ys n) m =
+  if m < n then nth None ys m else
+  if m < n + size xs then nth None xs (m - n) else nth None ys (m - size xs).
+Proof.
+  move => xs ys n; elim: n ys.
+  - move => /= ys m.
+    rewrite add0n subn0.
+    by elim: xs m => [| x xs IH] [].
+  - move => n IH [| y ys] [] //= m.
+    - by rewrite subSS addSn !ltnS IH !nth_nil.
+    - rewrite subSS addSn !ltnS IH.
+      (do 2 case: ifP => //) => H _.
+      rewrite subSn //; ssromega.
+Qed.
+
+Theorem ctxleq_refl : forall (xs : context), ctxleq xs xs.
+Proof.
+  done.
+Qed.
+
+Theorem ctxleq_trans :
+  forall (xs ys zs : context), ctxleq xs ys -> ctxleq ys zs -> ctxleq xs zs.
+Proof.
+  auto.
+Qed.
+
+Theorem ctxleq_nil : forall (xs : context), ctxleq [::] xs.
+Proof.
+  by move => xs n a; rewrite nth_nil.
+Qed.
+
+Theorem ctxleq_appl :
+  forall (xs ys zs : context), ctxleq ys zs -> ctxleq (xs ++ ys) (xs ++ zs).
+Proof.
+  by elim => // x xs IH ys zs H [] //=; apply IH.
+Qed.
+
+Theorem ctxleq_appr : forall (xs ys : context), ctxleq xs (xs ++ ys).
+Proof.
+  move => xs ys; elim: xs => // x xs.
+  - by rewrite nth_nil.
+  - by move => H [].
+Qed.
+
+Theorem ctxleq_app :
+  forall (xs xs' ys ys' : context), size xs = size xs' ->
+  ctxleq xs xs' -> ctxleq ys ys' -> ctxleq (xs ++ ys) (xs' ++ ys').
+Proof.
+  elim => [| x xs IH]; case => //= x' xs' ys ys' [H] H0 H1; case.
+  - move => /= a H2; apply (H0 0 a H2).
+  - move => /= n a; apply IH => // m; apply (H0 m.+1).
 Qed.
 
 (* Forall *)
@@ -61,3 +164,6 @@ Proof.
 Qed.
 
 End Seq.
+
+Notation ctxindex xs n x := (Some x = nth None xs n).
+Notation ctxleq xs ys := (forall n a, ctxindex xs n a -> ctxindex ys n a).
